Temporary fixes to Asm.v

riscV/Asm.v
@@ -1578,7 +1578,7 @@ Inductive step: state -> trace -> state -> Prop :=
       sig_call i = Some sig ->
       forall (NEXTPC: rs' PC = Vptr b' Ptrofs.zero), (* Only allow to call to ofs zero *)
       forall (NEXT_EXT: Genv.find_def ge b' = Some (Gfun (External ef))),
-      forall (ALLOWED: Genv.allowed_syscall ge cp ef),
+      forall (ALLOWED: Genv.allowed_syscall ge (comp_of f) ef),
 
 
       external_call ef ge (comp_of f) args m' t res m'' ->
@@ -1836,7 +1836,7 @@ Section ExecSem.
       possible_trace w t w' ->
       do_inline_assembly txt sg ge cp w vargs m = Some(w', t, vres, m').
 
-  Fixpoint get_builtin_arg (ge: genv) (rs: regset) (sp: val) (m: mem) (b: builtin_arg preg): option val :=
+  Fixpoint get_builtin_arg (ge: genv) (cp: compartment) (rs: regset) (sp: val) (m: mem) (b: builtin_arg preg): option val :=
     match b with
     | BA x => Some (rs x)
     | BA_int n => Some (Vint n)
@@ -1845,22 +1845,25 @@ Section ExecSem.
     | BA_single n => Some (Vsingle n)
     | BA_loadstack chunk ofs => Mem.loadv chunk m (Val.offset_ptr sp ofs) top
     | BA_addrstack ofs => Some (Val.offset_ptr sp ofs)
-    | BA_loadglobal chunk id ofs => Mem.loadv chunk m (Genv.symbol_address ge id ofs) top
-    | BA_addrglobal id ofs => Some (Genv.symbol_address ge id ofs)
+    | BA_loadglobal chunk id ofs =>
+          Mem.loadv chunk m (Genv.symbol_address ge id ofs) cp
+    | BA_addrglobal id ofs => if Genv.allowed_addrof_b ge cp id then
+                               Some (Genv.symbol_address ge id ofs)
+                             else None
     | BA_splitlong hi lo =>
-        match get_builtin_arg ge rs sp m hi, get_builtin_arg ge rs sp m lo with
+        match get_builtin_arg ge cp rs sp m hi, get_builtin_arg ge cp rs sp m lo with
         | Some vhi, Some vlo => Some (Val.longofwords vhi vlo)
         | _, _ => None
         end
     | BA_addptr a1 a2 =>
-        match get_builtin_arg ge rs sp m a1, get_builtin_arg ge rs sp m a2 with
+        match get_builtin_arg ge cp rs sp m a1, get_builtin_arg ge cp rs sp m a2 with
         | Some v1, Some v2 => Some (if Archi.ptr64 then Val.addl v1 v2 else Val.add v1 v2)
         | _, _ => None
         end
     end.
 
-  Lemma get_eval_builtin_arg: forall ge rs sp m b v,
-      get_builtin_arg ge rs sp m b = Some v <-> eval_builtin_arg ge rs sp m b v.
+  Lemma get_eval_builtin_arg: forall ge cp rs sp m b v,
+      get_builtin_arg ge cp rs sp m b = Some v <-> eval_builtin_arg ge cp rs sp m b v.
   Proof.
     intros until b.
     induction b; intros; simpl;
@@ -1868,32 +1871,37 @@ Section ExecSem.
     - split; [intros H; econstructor; eauto | intros H; inv H].
       destruct (Val.offset_ptr); try discriminate; simpl in *.
       eapply Mem.load_Some_None; eauto.
-    - split; [intros H; econstructor; eauto | intros H; inv H].
-      unfold Genv.symbol_address, Senv.symbol_address in *; simpl in *.
-      destruct (Genv.find_symbol ge id); try discriminate; simpl in *.
-      eapply Mem.load_Some_None; eauto.
+    - split; [intros H (* econstructor; eauto *) | intros H; inv H].
+      destruct Genv.allowed_addrof_b eqn:?. inv H.
+      econstructor; eauto. congruence.
+      destruct Genv.allowed_addrof_b eqn:?; auto.
+      rewrite H3 in Heqb; discriminate.
+      (* econstructor; eauto. congruence. *)
+      (* unfold Genv.symbol_address, Senv.symbol_address in *; simpl in *. *)
+      (* destruct (Genv.find_symbol ge id); try discriminate; simpl in *. *)
+      (* eapply Mem.load_Some_None; eauto. *)
     - split; [intros H | intros H; inv H].
-      + destruct (get_builtin_arg ge rs sp m b1); try discriminate.
-        destruct (get_builtin_arg ge rs sp m b2); try discriminate.
+      + destruct (get_builtin_arg ge cp rs sp m b1); try discriminate.
+        destruct (get_builtin_arg ge cp rs sp m b2); try discriminate.
         inv H. econstructor; [eapply IHb1 | eapply IHb2]; eauto.
       + now eapply IHb1 in H2; eapply IHb2 in H4;
           rewrite H2, H4.
     - split; [intros H | intros H; inv H].
-      + destruct (get_builtin_arg ge rs sp m b1); try discriminate.
-        destruct (get_builtin_arg ge rs sp m b2); try discriminate.
+      + destruct (get_builtin_arg ge cp rs sp m b1); try discriminate.
+        destruct (get_builtin_arg ge cp rs sp m b2); try discriminate.
         inv H. econstructor; [eapply IHb1 | eapply IHb2]; eauto.
       + now eapply IHb1 in H2; eapply IHb2 in H4;
           rewrite H2, H4.
   Qed.
 
-  Definition get_builtin_args' (ge: genv) (rs: regset) (v: val) (m: mem) (args: list (builtin_arg preg)): list (option val) :=
-    List.map (get_builtin_arg ge rs v m) args.
+  Definition get_builtin_args' (ge: genv) cp (rs: regset) (v: val) (m: mem) (args: list (builtin_arg preg)): list (option val) :=
+    List.map (get_builtin_arg ge cp rs v m) args.
 
-  Definition get_builtin_args ge rs v m args := list_option_option_list (get_builtin_args' ge rs v m args).
+  Definition get_builtin_args ge cp rs v m args := list_option_option_list (get_builtin_args' ge cp rs v m args).
 
 
-  Lemma get_eval_builtin_args: forall ge rs sp m bl vl,
-      get_builtin_args ge rs sp m bl = Some vl <-> eval_builtin_args ge rs sp m bl vl.
+  Lemma get_eval_builtin_args: forall ge cp rs sp m bl vl,
+      get_builtin_args ge cp rs sp m bl = Some vl <-> eval_builtin_args ge cp rs sp m bl vl.
   Proof.
     intros until bl.
     induction bl; intros.
@@ -1901,11 +1909,11 @@ Section ExecSem.
       split; intros H; inv H; [constructor | reflexivity].
     - unfold get_builtin_args; simpl.
       split.
-      + intros H. destruct (get_builtin_arg ge rs sp m a) eqn:get_a.
-        * destruct (list_option_option_list (get_builtin_args' ge rs sp m bl)) eqn:get_rest; try discriminate.
+      + intros H. destruct (get_builtin_arg ge cp rs sp m a) eqn:get_a.
+        * destruct (list_option_option_list (get_builtin_args' ge cp rs sp m bl)) eqn:get_rest; try discriminate.
           inv H.
           constructor; [eapply get_eval_builtin_arg; eauto | eapply IHbl; exact get_rest].
-        * destruct (list_option_option_list (get_builtin_args' ge rs sp m bl)); discriminate.
+        * destruct (list_option_option_list (get_builtin_args' ge cp rs sp m bl)); discriminate.
       + intros H.
         inv H.
         eapply get_eval_builtin_arg in H2; rewrite H2.
@@ -1913,132 +1921,131 @@ Section ExecSem.
         unfold get_builtin_args in IHbl2. rewrite IHbl2; auto.
   Qed.
 
+  (* Definition take_step (p: program) (ge: genv) (w: world) (s: state): option (trace * state) := *)
+  (*   let comp_of_main := comp_of_main p in *)
+  (*   match s with *)
+  (*   | State st rs m cp => *)
+  (*       do Vptr b ofs <- rs PC; *)
+  (*       do fd <- Genv.find_funct_ptr ge b; *)
+  (*       match fd with *)
+  (*       | Internal f => *)
+  (*           do i <- find_instr (Ptrofs.unsigned ofs) (fn_code f); *)
+  (*           match i with *)
+  (*           | Pbuiltin ef args res => *)
+  (*               do vargs <- get_builtin_args ge rs (rs X2) m args; *)
+  (*               do res_builtin <- do_external _ _ ge do_external_function do_inline_assembly ef cp w vargs m; *)
+  (*               check (Genv.allowed_syscall_b ge (comp_of f) ef); *)
+  (*               let '(w', t, vres, m') := res_builtin in *)
+  (*               let rs' := nextinstr *)
+  (*                         (set_res res vres (undef_regs (map preg_of (destroyed_by_builtin ef)) (rs # X1 <- Vundef) # X31 <- Vundef)) in *)
+  (*               Some (t, State st rs' m' (comp_of f)) *)
+  (*           | _ => *)
+  (*               match exec_instr ge f i rs m (comp_of f) with *)
+  (*               | Next rs' m' => *)
+  (*                   match sig_call i, is_return i with *)
+  (*                   | None, false => (* exec_step_internal *) *)
+  (*                       do Vptr b' ofs' <- rs' PC; *)
+  (*                       let cp' := Genv.find_comp_of_block ge b' in *)
+  (*                       check (cp_eq_dec (comp_of f) cp'); *)
+  (*                       Some (E0, State st rs' m' (comp_of f)) *)
+  (*                   | Some sig, false => (* exec_step_internal_call *) *)
+  (*                       do Vptr b' ofs' <- rs' PC; *)
+  (*                       check (Genv.allowed_call_b ge (comp_of f) (Vptr b' Ptrofs.zero)); *)
+  (*                       do st' <- update_stack_call ge st sig (comp_of f) rs'; *)
+  (*                       do vargs <- get_call_arguments rs' m' sig; *)
+  (*                       let cp' := Genv.find_comp_of_block ge b' in *)
+  (*                       check (match Genv.type_of_call (comp_of f) cp' with *)
+  (*                              | Genv.CrossCompartmentCall => forallb not_ptr_b vargs *)
+  (*                              | _ => true *)
+  (*                              end); *)
+  (*                       do t <- get_call_trace _ _ ge (comp_of f) cp' (Vptr b' ofs') vargs (sig_args sig); *)
+  (*                       Some (t, State st' rs' m' (comp_of f)) *)
+  (*                   | None, true => (* exec_step_internal_return *) *)
+  (*                       (* check (Genv.allowed_call_b ge (comp_of f) (rs' PC)); *) *)
+  (*                       Some (E0, ReturnState st rs' m' (comp_of f)) *)
+  (*                   | Some _, true => None *)
+  (*                   end *)
+  (*               | Stuck => None *)
+  (*               end *)
+  (*           end *)
+  (*       | External ef => *)
+  (*           check (Ptrofs.eq ofs Ptrofs.zero); *)
+  (*           do vargs <- get_extcall_arguments rs m (ef_sig ef); *)
+  (*           do res_external <- do_external _ _ ge do_external_function do_inline_assembly ef cp w vargs m; *)
+  (*           check (Genv.allowed_syscall_b ge cp ef); *)
+  (*           let '(w', t, res, m') := res_external in *)
+  (*           let rs' := (set_pair (loc_external_result (ef_sig ef)) res (undef_caller_save_regs rs)) # PC <- (rs X1) in *)
+  (*           Some (t, ReturnState st rs' m' bottom) *)
+  (*       end *)
+  (*   | ReturnState st rs m rec_cp => *)
+  (*       check (negb (Val.eq (rs PC) Vnullptr)); *)
+  (*       let cp' := Genv.find_comp_in_genv ge (rs PC) in *)
 
-  Definition take_step (p: program) (ge: genv) (w: world) (s: state): option (trace * state) :=
-    let comp_of_main := comp_of_main p in
-    match s with
-    | State st rs m cp =>
-        do Vptr b ofs <- rs PC;
-        do fd <- Genv.find_funct_ptr ge b;
-        match fd with
-        | Internal f =>
-            do i <- find_instr (Ptrofs.unsigned ofs) (fn_code f);
-            match i with
-            | Pbuiltin ef args res =>
-                do vargs <- get_builtin_args ge rs (rs X2) m args;
-                do res_builtin <- do_external _ _ ge do_external_function do_inline_assembly ef cp w vargs m;
-                check (Genv.allowed_syscall_b ge (comp_of f) ef);
-                let '(w', t, vres, m') := res_builtin in
-                let rs' := nextinstr
-                          (set_res res vres (undef_regs (map preg_of (destroyed_by_builtin ef)) (rs # X1 <- Vundef) # X31 <- Vundef)) in
-                Some (t, State st rs' m' (comp_of f))
-            | _ =>
-                match exec_instr ge f i rs m (comp_of f) with
-                | Next rs' m' =>
-                    match sig_call i, is_return i with
-                    | None, false => (* exec_step_internal *)
-                        do Vptr b' ofs' <- rs' PC;
-                        let cp' := Genv.find_comp_of_block ge b' in
-                        check (cp_eq_dec (comp_of f) cp');
-                        Some (E0, State st rs' m' (comp_of f))
-                    | Some sig, false => (* exec_step_internal_call *)
-                        do Vptr b' ofs' <- rs' PC;
-                        check (Genv.allowed_call_b ge (comp_of f) (Vptr b' Ptrofs.zero));
-                        do st' <- update_stack_call ge st sig (comp_of f) rs';
-                        do vargs <- get_call_arguments rs' m' sig;
-                        let cp' := Genv.find_comp_of_block ge b' in
-                        check (match Genv.type_of_call (comp_of f) cp' with
-                               | Genv.CrossCompartmentCall => forallb not_ptr_b vargs
-                               | _ => true
-                               end);
-                        do t <- get_call_trace _ _ ge (comp_of f) cp' (Vptr b' ofs') vargs (sig_args sig);
-                        Some (t, State st' rs' m' (comp_of f))
-                    | None, true => (* exec_step_internal_return *)
-                        (* check (Genv.allowed_call_b ge (comp_of f) (rs' PC)); *)
-                        Some (E0, ReturnState st rs' m' (comp_of f))
-                    | Some _, true => None
-                    end
-                | Stuck => None
-                end
-            end
-        | External ef =>
-            check (Ptrofs.eq ofs Ptrofs.zero);
-            do vargs <- get_extcall_arguments rs m (ef_sig ef);
-            do res_external <- do_external _ _ ge do_external_function do_inline_assembly ef cp w vargs m;
-            check (Genv.allowed_syscall_b ge cp ef);
-            let '(w', t, res, m') := res_external in
-            let rs' := (set_pair (loc_external_result (ef_sig ef)) res (undef_caller_save_regs rs)) # PC <- (rs X1) in
-            Some (t, ReturnState st rs' m' bottom)
-        end
-    | ReturnState st rs m rec_cp =>
-        check (negb (Val.eq (rs PC) Vnullptr));
-        let cp' := Genv.find_comp_in_genv ge (rs PC) in
+  (*       (* let rec_cp' := call_comp ge st in *) *)
+  (*       check (match flowsto_dec rec_cp cp' with *)
+  (*              | left _ => true *)
+  (*              | right _ => andb (Val.eq (rs PC) (asm_parent_ra st)) (Val.eq (rs X2) (asm_parent_sp st)) *)
+  (*              end); *)
+  (*       do st' <- update_stack_return ge st rec_cp rs; *)
+  (*       let sg := sig_of_call st in *)
+  (*       check (match Genv.type_of_call cp' rec_cp with *)
+  (*              | Genv.CrossCompartmentCall => not_ptr_b (return_value rs sg) *)
+  (*              | _ => true end); *)
+  (*       do t <- get_return_trace _ _ ge cp' rec_cp (return_value rs sg) (sig_res sg); *)
+  (*       Some (t, State st' rs m cp') *)
+  (*   end. *)
 
-        (* let rec_cp' := call_comp ge st in *)
-        check (match flowsto_dec rec_cp cp' with
-               | left _ => true
-               | right _ => andb (Val.eq (rs PC) (asm_parent_ra st)) (Val.eq (rs X2) (asm_parent_sp st))
-               end);
-        do st' <- update_stack_return ge st rec_cp rs;
-        let sg := sig_of_call st in
-        check (match Genv.type_of_call cp' rec_cp with
-               | Genv.CrossCompartmentCall => not_ptr_b (return_value rs sg)
-               | _ => true end);
-        do t <- get_return_trace _ _ ge cp' rec_cp (return_value rs sg) (sig_res sg);
-        Some (t, State st' rs m cp')
-    end.
+  (* Definition at_final_state (s: state): option int := *)
+  (*   match s with *)
+  (*   | ReturnState nil rs m cp => *)
+  (*       match rs X10 with *)
+  (*       | Vint r => if Val.eq (rs PC) Vnullptr then Some r else None *)
+  (*       | _ => None *)
+  (*       end *)
+  (*   | _ => None *)
+  (*   end. *)
 
-  Definition at_final_state (s: state): option int :=
-    match s with
-    | ReturnState nil rs m cp =>
-        match rs X10 with
-        | Vint r => if Val.eq (rs PC) Vnullptr then Some r else None
-        | _ => None
-        end
-    | _ => None
-    end.
-
-  Lemma take_step_correct: forall p w s t s',
-      let ge := Genv.globalenv p in
-      step ge s t s' ->
-      take_step p ge w s = Some (t, s').
-  Proof.
-    intros p w s t s' ge H.
-    inv H; simpl; eauto.
-    - rewrite H0, H1, H2, H3, H4, H5, NEXTPC, ALLOWED.
-      destruct cp_eq_dec; try congruence. destruct i; auto. inv H3.
-    - rewrite H0, H1, H2, H3, H4, NEXTPC.
-      destruct i; inv H4; simpl.
-      + apply Genv.allowed_call_reflect in ALLOWED; rewrite ALLOWED.
-        rewrite STUPD. eapply get_call_arguments_equiv in ARGS; eauto; rewrite ARGS.
-        simpl in NO_CROSS_PTR. destruct flowsto_dec; try auto.
-        * apply get_call_trace_eq in EV; rewrite EV. reflexivity.
-        * exploit NO_CROSS_PTR; eauto; intros G.
-          rewrite Forall_forall in G.
-          pose proof forallb_forall as [X Y]. rewrite Y.
-          apply get_call_trace_eq in EV; rewrite EV. reflexivity.
-          intros. exploit G; eauto. intros. eapply not_ptr_reflect; eauto.
-      + apply Genv.allowed_call_reflect in ALLOWED; rewrite ALLOWED.
-        rewrite STUPD. eapply get_call_arguments_equiv in ARGS; eauto; rewrite ARGS.
-        simpl in NO_CROSS_PTR. destruct flowsto_dec; try auto.
-        * apply get_call_trace_eq in EV; rewrite EV. reflexivity.
-        * exploit NO_CROSS_PTR; eauto; intros G.
-          rewrite Forall_forall in G.
-          pose proof forallb_forall as [X Y]. rewrite Y.
-          apply get_call_trace_eq in EV; rewrite EV. reflexivity.
-          intros. exploit G; eauto. intros. eapply not_ptr_reflect; eauto.
-    - rewrite H0, H1, H2, H3, H4.
-      destruct i; inv H4; simpl. reflexivity.
-    - destruct Val.eq; try congruence; simpl in *.
-      rewrite STUPD. apply get_return_trace_eq in EV. rewrite EV.
-      destruct flowsto_dec; simpl; auto.
-      rewrite RESTORE_SP, PC_RA; eauto.
-      do 2 destruct Val.eq; try contradiction. simpl.
-      exploit NO_CROSS_PTR; eauto; intros G.
-      apply not_ptr_reflect in G; rewrite G. reflexivity.
-    - admit.
-    - admit.
-  Admitted.
+  (* Lemma take_step_correct: forall p w s t s', *)
+  (*     let ge := Genv.globalenv p in *)
+  (*     step ge s t s' -> *)
+  (*     take_step p ge w s = Some (t, s'). *)
+  (* Proof. *)
+  (*   intros p w s t s' ge H. *)
+  (*   inv H; simpl; eauto. *)
+  (*   - rewrite H0, H1, H2, H3, H4, H5, NEXTPC, ALLOWED. *)
+  (*     destruct cp_eq_dec; try congruence. destruct i; auto. inv H3. *)
+  (*   - rewrite H0, H1, H2, H3, H4, NEXTPC. *)
+  (*     destruct i; inv H4; simpl. *)
+  (*     + apply Genv.allowed_call_reflect in ALLOWED; rewrite ALLOWED. *)
+  (*       rewrite STUPD. eapply get_call_arguments_equiv in ARGS; eauto; rewrite ARGS. *)
+  (*       simpl in NO_CROSS_PTR. destruct flowsto_dec; try auto. *)
+  (*       * apply get_call_trace_eq in EV; rewrite EV. reflexivity. *)
+  (*       * exploit NO_CROSS_PTR; eauto; intros G. *)
+  (*         rewrite Forall_forall in G. *)
+  (*         pose proof forallb_forall as [X Y]. rewrite Y. *)
+  (*         apply get_call_trace_eq in EV; rewrite EV. reflexivity. *)
+  (*         intros. exploit G; eauto. intros. eapply not_ptr_reflect; eauto. *)
+  (*     + apply Genv.allowed_call_reflect in ALLOWED; rewrite ALLOWED. *)
+  (*       rewrite STUPD. eapply get_call_arguments_equiv in ARGS; eauto; rewrite ARGS. *)
+  (*       simpl in NO_CROSS_PTR. destruct flowsto_dec; try auto. *)
+  (*       * apply get_call_trace_eq in EV; rewrite EV. reflexivity. *)
+  (*       * exploit NO_CROSS_PTR; eauto; intros G. *)
+  (*         rewrite Forall_forall in G. *)
+  (*         pose proof forallb_forall as [X Y]. rewrite Y. *)
+  (*         apply get_call_trace_eq in EV; rewrite EV. reflexivity. *)
+  (*         intros. exploit G; eauto. intros. eapply not_ptr_reflect; eauto. *)
+  (*   - rewrite H0, H1, H2, H3, H4. *)
+  (*     destruct i; inv H4; simpl. reflexivity. *)
+  (*   - destruct Val.eq; try congruence; simpl in *. *)
+  (*     rewrite STUPD. apply get_return_trace_eq in EV. rewrite EV. *)
+  (*     destruct flowsto_dec; simpl; auto. *)
+  (*     rewrite RESTORE_SP, PC_RA; eauto. *)
+  (*     do 2 destruct Val.eq; try contradiction. simpl. *)
+  (*     exploit NO_CROSS_PTR; eauto; intros G. *)
+  (*     apply not_ptr_reflect in G; rewrite G. reflexivity. *)
+  (*   - admit. *)
+  (*   - admit. *)
+  (* Admitted. *)
 
 Definition build_initial_state (p: program): option state :=
   let ge := Genv.globalenv p in
